code/k256/Hacl.K256.ECDSA.fst
@@ -28,21 +28,23 @@ let lbytes32 = lbuffer uint8 32ul
 
 
 inline_for_extraction noextract
-val ecdsa_sign_r: r:qelem -> k:lbytes32 -> Stack unit
-  (requires fun h -> live h r /\ live h k /\ disjoint r k)
+val ecdsa_sign_r (r k:qelem) : Stack unit
+  (requires fun h ->
+    live h r /\ live h k /\ disjoint r k /\
+    qas_nat h k < S.q)
   (ensures fun h0 _ h1 -> modifies (loc r) h0 h1 /\
-   (let _X, _Y, _Z = S.point_mul_g (as_seq h0 k) in
+   (let _X, _Y, _Z = S.point_mul_g (qas_nat h0 k) in
     let x = S.fmul _X (S.finv _Z) in
     let r_s = x % S.q in
     qas_nat h1 r == r_s))
 
 let ecdsa_sign_r r k =
   push_frame ();
-  let p = create (3ul *! nlimb) (u64 0) in
-  let x, y, z = getx p, gety p, getz p in
   let tmp = create_felem () in
-
+  let p = create_point () in
   point_mul_g p k; // p = [k]G
+  let x, y, z = getx p, gety p, getz p in
+
   finv tmp z; // tmp = zinv
   fmul tmp x tmp; // tmp = aff_x = x *% zinv
   qelem_from_felem r tmp; // r = aff_x % S.q
@@ -50,24 +52,24 @@ let ecdsa_sign_r r k =
 
 
 inline_for_extraction noextract
-val ecdsa_sign_s (s:qelem) (m private_key k:lbytes32) (r:qelem) : Stack unit
+val ecdsa_sign_s (s k r:qelem) (m private_key:lbytes32) : Stack unit
   (requires fun h ->
     live h s /\ live h m /\ live h private_key /\
-    live h k /\ live h r /\ disjoint s r /\
+    live h k /\ live h r /\
+    disjoint s r /\ disjoint s k /\ disjoint r k /\
 
-   (let sk_nat = BSeq.nat_from_bytes_be (as_seq h private_key) in
-    let k_nat = BSeq.nat_from_bytes_be (as_seq h k) in
-    0 < sk_nat /\ sk_nat < S.q /\
-    0 < k_nat /\ k_nat < S.q /\
-    qas_nat h r < S.q))
+    0 < qas_nat h k /\ qas_nat h k < S.q /\
+    qas_nat h r < S.q /\
+   (let d_a = BSeq.nat_from_bytes_be (as_seq h private_key) in
+    0 < d_a /\ d_a < S.q))
   (ensures fun h0 _ h1 -> modifies (loc s) h0 h1 /\
    (let z = BSeq.nat_from_bytes_be (as_seq h0 m) % S.q in
     let d_a = BSeq.nat_from_bytes_be (as_seq h0 private_key) in
-    let kinv = S.qinv (BSeq.nat_from_bytes_be (as_seq h0 k)) in
+    let kinv = S.qinv (qas_nat h0 k) in
     let s_s = S.qmul kinv (S.qadd z (S.qmul (qas_nat h0 r) d_a)) in
     qas_nat h1 s == s_s))
 
-let ecdsa_sign_s s m private_key k r =
+let ecdsa_sign_s s k r m private_key =
   push_frame ();
   let z = create_qelem () in
   let d_a = create_qelem () in
@@ -75,8 +77,7 @@ let ecdsa_sign_s s m private_key k r =
 
   load_qelem_modq z m; // z = m % S.q
   load_qelem d_a private_key; // d_a = private_key
-  load_qelem kinv k;
-  qinv kinv kinv;
+  qinv kinv k;
 
   qmul s r d_a; // s = r * d_a
   qadd s z s; // s = z + s
@@ -89,9 +90,11 @@ let ecdsa_sign_hashed_msg r s m private_key k =
   push_frame ();
   let r_q = create_qelem () in
   let s_q = create_qelem () in
+  let k_q = create_qelem () in
 
-  ecdsa_sign_r r_q k;
-  ecdsa_sign_s s_q m private_key k r_q;
+  load_qelem k_q k;
+  ecdsa_sign_r r_q k_q;
+  ecdsa_sign_s s_q k_q r_q m private_key;
 
   store_qelem r r_q;
   store_qelem s s_q;
@@ -103,9 +106,81 @@ let ecdsa_sign_hashed_msg r s m private_key k =
   b
 
 
+inline_for_extraction noextract
+val ecdsa_verify_qelem (res p:point) (z r s:qelem) : Stack unit
+  (requires fun h ->
+    live h res /\ live h p /\ live h z /\ live h r /\ live h s /\
+    disjoint res p /\ point_inv h p /\
+    qas_nat h z < S.q /\ qas_nat h r < S.q /\ qas_nat h s < S.q)
+  (ensures  fun h0 _ h1 -> modifies (loc res) h0 h1 /\ point_inv h1 res /\
+    (let sinv = S.qinv (qas_nat h0 s) in
+     let u1 = S.qmul (qas_nat h0 z) sinv in
+     let u2 = S.qmul (qas_nat h0 r) sinv in
+     S.to_aff_point (point_as_nat3_proj h1 res) ==
+     S.to_aff_point (S.point_mul_double_g u1 u2 (point_as_nat3_proj h0 p))))
+
+let ecdsa_verify_qelem res p z r s =
+  push_frame ();
+  let sinv = create_qelem () in
+  let u1 = create_qelem () in
+  let u2 = create_qelem () in
+
+  qinv sinv s;
+  qmul u1 z sinv;
+  qmul u2 r sinv;
+  point_mul_g_double_vartime res u1 u2 p;
+  pop_frame ()
+
+
+inline_for_extraction noextract
+val ecdsa_verify_qelem_aff (public_key:aff_point) (z r s:qelem) : Stack bool
+  (requires fun h ->
+    live h public_key /\ live h z /\ live h r /\ live h s /\
+    aff_point_inv h public_key /\
+    qas_nat h z < S.q /\ qas_nat h r < S.q /\ qas_nat h s < S.q)
+  (ensures  fun h0 b h1 -> modifies0 h0 h1 /\
+    (let sinv = S.qinv (qas_nat h0 s) in
+     let u1 = S.qmul (qas_nat h0 z) sinv in
+     let u2 = S.qmul (qas_nat h0 r) sinv in
+     let p = S.to_proj_point (aff_point_as_nat2_aff h0 public_key) in
+     let _X, _Y, _Z = S.point_mul_double_g u1 u2 p in
+     b = (S.fmul _X (S.finv _Z) % S.q = (qas_nat h0 r))))
+
+let ecdsa_verify_qelem_aff public_key z r s =
+  push_frame ();
+  let p = create_point () in
+  let res = create_point () in
+  let zinv = create_felem () in
+  let xq = create_qelem () in
+
+  to_proj_point p public_key;
+  ecdsa_verify_qelem res p z r s;
+  let _X, _Y, _Z = getx res, gety res, getz res in
+
+  finv zinv _Z;
+  fmul zinv _X zinv;
+  qelem_from_felem xq zinv;
+  let b = is_qelem_eq_vartime xq r in
+  pop_frame ();
+  b
+
+
 [@CInline]
 let ecdsa_verify_hashed_msg m public_key r s =
-  admit()
+  push_frame ();
+  let r_q = create_qelem () in
+  let s_q = create_qelem () in
+  let z = create_qelem () in
+
+  let is_r_valid = load_qelem_vartime r_q r in
+  let is_s_valid = load_qelem_vartime s_q s in
+  load_qelem_modq z m;
+
+  let res =
+    if not (is_r_valid && is_s_valid) then false
+    else ecdsa_verify_qelem_aff public_key z r_q s_q in
+  pop_frame ();
+  res
 
 
 [@CInline]
